Reasoning lemmas about the handlers

src/coq/Handlers/Memory.v
@@ -10,7 +10,7 @@
 
 
 From Coq Require Import
-     ZArith List String Omega
+     Morphisms ZArith List String Omega
      FSets.FMapAVL
      Structures.OrderedTypeEx
      ZMicromega.
@@ -731,14 +731,112 @@ Admitted.
     Context `{FailureE -< F} `{UBE -< F} `{PickE -< F}.
     Notation Effin := (E +' IntrinsicE +' MemoryE +' F).
     Notation Effout := (E +' F).
-    Notation Effin' := (E +' G +' IntrinsicE +' MemoryE +' F).
-    Notation Effout' := (E +' G +' F).
 
     Definition E_trigger {M} : forall R, E R -> (stateT M (itree Effout) R) :=
       fun R e m => r <- trigger e ;; ret (m, r).
 
     Definition F_trigger {M} : forall R, F R -> (stateT M (itree Effout) R) :=
       fun R e m => r <- trigger e ;; ret (m, r).
+
+    Definition interp_memory_h := case_ E_trigger (case_ handle_intrinsic  (case_ handle_memory  F_trigger)).
+    Definition interp_memory :
+      itree Effin ~> stateT memory_stack (itree Effout) :=
+      interp_state interp_memory_h.
+
+    Section Structural_Lemmas.
+      
+      Lemma interp_memory_bind :
+        forall (R S : Type) (t : itree Effin R) (k : R -> itree Effin S) m,
+          interp_memory (ITree.bind t k) m ≅
+                        ITree.bind (interp_memory t m) (fun '(m',r) => interp_memory (k r) m').
+      Proof.
+        intros.
+        unfold interp_memory.
+        setoid_rewrite interp_state_bind.
+        apply eq_itree_clo_bind with (UU := Logic.eq).
+        reflexivity.
+        intros [] [] EQ; inv EQ; reflexivity.
+      Qed.
+
+      Lemma interp_memory_ret :
+        forall (R : Type) g (x: R),
+          interp_memory (Ret x: itree Effin R) g ≅ Ret (g,x).
+      Proof.
+        intros; apply interp_state_ret.
+      Qed.
+
+      Lemma interp_memory_vis_eqit:
+        forall S X (kk : X -> itree Effin S) m
+          (e : Effin X),
+          interp_memory (Vis e kk) m ≅ ITree.bind (interp_memory_h e m) (fun sx => Tau (interp_memory (kk (snd sx)) (fst sx))).
+      Proof.
+        intros.
+        unfold interp_memory.
+        setoid_rewrite interp_state_vis.
+        reflexivity.
+      Qed.
+
+      Lemma interp_memory_vis:
+        forall m S X (kk : X -> itree Effin S) (e : Effin X),
+          interp_memory (Vis e kk) m ≈ ITree.bind (interp_memory_h e m) (fun sx => interp_memory (kk (snd sx)) (fst sx)).
+      Proof.
+        intros.
+        rewrite interp_memory_vis_eqit.
+        apply eutt_eq_bind.
+        intros ?; tau_steps; reflexivity.
+      Qed.
+
+      Lemma interp_memory_trigger:
+        forall (m : memory_stack) X (e : Effin X),
+          interp_memory (ITree.trigger e) m ≈ interp_memory_h e m. 
+      Proof.
+        intros.
+        unfold interp_memory.
+        rewrite interp_state_trigger.
+        reflexivity.
+      Qed.
+
+      Lemma interp_memory_bind_trigger_eqit:
+        forall m S X (kk : X -> itree Effin S) (e : Effin X),
+          interp_memory (ITree.bind (trigger e) kk) m ≅ ITree.bind (interp_memory_h e m) (fun sx => Tau (interp_memory (kk (snd sx)) (fst sx))).
+      Proof.
+        intros.
+        unfold interp_memory.
+        rewrite bind_trigger.
+        setoid_rewrite interp_state_vis.
+        reflexivity.
+      Qed.
+
+      Lemma interp_memory_bind_trigger:
+        forall m S X
+          (kk : X -> itree Effin S)
+          (e : Effin X),
+          interp_memory (ITree.bind (trigger e) kk) m ≈ ITree.bind (interp_memory_h e m) (fun sx => interp_memory (kk (snd sx)) (fst sx)).
+      Proof.
+        intros.
+        rewrite interp_memory_bind_trigger_eqit.
+        apply eutt_eq_bind.
+        intros ?; tau_steps; reflexivity.
+      Qed.
+
+      Global Instance eutt_interp_memory {R} :
+        Proper (eutt Logic.eq ==> Logic.eq ==> eutt Logic.eq) (@interp_memory R). 
+      Proof.
+        repeat intro.
+        unfold interp_memory. 
+        subst; rewrite H2.
+        reflexivity.
+      Qed.
+
+    End Structural_Lemmas.
+
+
+  (** ** DEPRECATED
+        TODO : Double check, garbage collect
+   *)
+  (*
+    Notation Effin' := (E +' G +' IntrinsicE +' MemoryE +' F).
+    Notation Effout' := (E +' G +' F).
 
     Definition E_trigger' {M} : forall R, E R -> (stateT M (itree Effout') R) :=
       fun R e m => r <- trigger e ;; ret (m, r).
@@ -749,33 +847,9 @@ Admitted.
     Definition G_trigger' {M} : forall R, G R -> (stateT M (itree Effout') R) :=
       fun R e m => r <- trigger e ;; ret (m, r).
 
-    Definition interp_memory :
-      itree Effin ~> stateT memory_stack (itree Effout) :=
-      interp_state (case_ E_trigger  (case_ handle_intrinsic  (case_ handle_memory  F_trigger))).
-
     Definition interp_memory' :
       itree Effin' ~> stateT memory_stack (itree Effout') :=
       interp_state (case_ E_trigger' (case_ G_trigger' (case_ handle_intrinsic (case_ handle_memory F_trigger')))).
-
-    Lemma interp_memory_bind :
-      forall (R S : Type) (t : itree Effin R) (k : R -> itree Effin S) m,
-        interp_memory (ITree.bind t k) m ≅
-         ITree.bind (interp_memory t m) (fun '(m',r) => interp_memory (k r) m').
-    Proof.
-      intros.
-      unfold interp_memory.
-      setoid_rewrite interp_state_bind.
-      apply eq_itree_clo_bind with (UU := Logic.eq).
-      reflexivity.
-      intros [] [] EQ; inv EQ; reflexivity.
-    Qed.
-
-    Lemma interp_memory_ret :
-      forall (R : Type) g (x: R),
-        interp_memory (Ret x: itree Effin R) g ≅ Ret (g,x).
-    Proof.
-      intros; apply interp_state_ret.
-    Qed.
 
     Lemma interp_memory'_bind :
       forall (R S : Type) (t : itree Effin' R) (k : R -> itree Effin' S) m,
@@ -796,6 +870,9 @@ Admitted.
     Proof.
       intros; apply interp_state_ret.
     Qed.
+
+
+   *)
 
   End PARAMS.
 
